Publish previews: main 9af2ebb6, 9 PRs, 2 unavailable
Main: 9af2ebb6

Pull requests:
- PR #171: published at a5930f90 (9 changed variants)
- PR #179: published at ee0b7294 (9 changed variants)
- PR #181: published at 7e02bb1d (9 changed variants)
- PR #185: published at b7729749 (9 changed variants)
- PR #186: waiting-ci at 673368c6
- PR #203: published at 57223e7f (9 changed variants)
- PR #213: published at 6dffff89 (9 changed variants)
- PR #214: published at 860a2bdc (9 changed variants)
- PR #216: ci-failed at 05b36c22
- PR #218: published at deba7c05 (9 changed variants)
- PR #224: published at 82e1789f (9 changed variants)

pr/179/head/lf/terse/html-multi/-verso-search/searchIndex_141.2d136e7ed4a3704f.js
@@ -1,0 +1,1 @@
+window.docContents[141].resolve({"/UsingLean/#UsingLean":{"contents":"Chapter goals:\nNats\ndsimp\ncalc\n\n\n\nDid we intend for this section header to be in a \"full\" block?\n\n\n\n\n\n\n\n\n\n\n\n\n\n","context":"Logical Foundations","header":"4. UsingLean: Using the full power of a proof assistant","id":"/UsingLean/#UsingLean"}});
